---
layout: post
title: Integral 3
description: wut
summary: wut
comments: false
---

Show that:

$$
\int_0^1 s^a (1-s^2)^b ds = \frac{1}{2}\frac{\Gamma\big((a+1)/2\big) \Gamma\big(b+1\big)}{\Gamma\big((a+1)/2 + b + 1\big)},
$$

where

$$
a, b > 1.
$$

Solution:

Recalling again that

$$
B(p,q) = 2\int_0^{\pi/2} (\cos x)^{2p-1} (\sin x)^{2q-1} dx
$$

$$
= \frac{\Gamma\big(p\big) \Gamma\big(q\big)}{\Gamma\big(p+q\big)}
$$

for (in particular):

$$
p, q > 0.
$$

And making the change

$$
(\cos x)^2 \to u
$$

we have

$$
B(p,q) = 2\int_0^{\pi/2} (\cos x)^{2(p-1)} (\sin x)^{2(q-1)} \cos x \sin x dx =
$$

$$
= 2\int_0^{\pi/2} (\cos x)^{2(p-1)} (1 - (\cos x)^2)^{q-1} \cos x \sin x dx =
$$

$$
= \int_0^1 u^{p-1}(1-u)^{q-1}du.
$$

So, changing the variable

$$
s^2 \to t
$$

in the integral

$$
I = \int_0^1 s^a (1-s^2)^b ds 
$$

we have:

$$
\frac{1}{2}\int_0^1 s^{a-1}(1-s^2)^b 2sds = 
$$

$$
= \frac{1}{2}\int_0^1 t^{(a-1)/2}(1-t)^bdt,
$$

therefore, for

$$
p-1 = (a-1)/2, ~~~ q-1 = b
$$

which we can do since

$$
a, b > 1,
$$

we can identify the integral I with B(p,q):

$$
I = \frac{1}{2}B\Big((a+1)/2, b+1\Big) =
$$

$$
= \frac{1}{2}\frac{\Gamma\big((a+1)/2\big) \Gamma\big(b+1\big)}{\Gamma\big((a+1)/2 + b + 1\big)}.
$$

Qed.
